theories/models/utp_cml/utp_cml_monad.thy
@@ -8,8 +8,26 @@ header {* CML Monad *}
 
 theory utp_cml_monad
 imports 
-  utp_cml_expr
+  utp_cml_sorts
 begin
+
+(* CML expressions and CML predicates *)
+
+type_synonym 'a cmle        = "('a option, cmlv) pexpr"
+type_synonym cmlb           = "cmlv binding"
+type_synonym cmlp           = "cmlv upred" 
+type_synonym 'a cmlvar      = "('a option, cmlv) pvar"
+type_synonym ('a, 'b) cmlop = "('a option, 'b option, cmlv) WF_POPERATION"
+type_synonym cmlev          = "cmlv EVENT"
+type_synonym 'a cmlch       = "'a CHAN"
+
+translations
+  (type) "'a cmle" <= (type) "('a option, cmlv) pexpr"
+  (type) "cmlb" <= (type) "cmlv binding"
+  (type) "cmlp" <= (type) "cmlv upred"
+  (type) "'a cmlvar" <= (type) "('a option, cmlv) pvar"
+  (type) "('a, 'b) cmlop" <= (type) "'a cmle \<Rightarrow> 'b cmlvar \<times> bool \<Rightarrow> cmlp"
+  (type) "cmlev" <= (type) "cmlv EVENT"
 
 text {* Monadic bind for finite sets *}
 
