theories/models/utp_cml/utp_cml_process.thy
@@ -27,9 +27,47 @@ definition CMLOpO ::
 
 declare CMLOpO_def [uop_defs]
 
+term "MkVarD"
+
+definition ForLoopSetD :: "'a fset cmle \<Rightarrow> ('a option \<Rightarrow> cmlp) \<Rightarrow> cmlp" where
+"ForLoopSetD xs F = undefined"
+
 definition ParallelD :: 
-  "cmlp \<Rightarrow> cmlv UCHAN set \<Rightarrow> cmlp \<Rightarrow> cmlp" where
-"ParallelD p cs q = ParallelCSP p (LitPE (Abs_USET (MkEvents cs))) q"
+  "cmlp \<Rightarrow> cmlev set \<Rightarrow> cmlp \<Rightarrow> cmlp" where
+"ParallelD p cs q = ParallelCSP p (LitPE (Abs_USET cs)) q"
+
+definition AlphaSeqSetD ::
+  "'a fset cmle \<Rightarrow> ('a option \<Rightarrow> cmlp) \<Rightarrow> cmlp" where
+"AlphaSeqSetD = undefined"
+
+definition AlphaIntSetD ::
+  "'a fset cmle \<Rightarrow> ('a option \<Rightarrow> cmlp) \<Rightarrow> cmlp" where
+"AlphaIntSetD = undefined"
+
+definition AlphaExtSetD ::
+  "'a fset cmle \<Rightarrow> ('a option \<Rightarrow> cmlp) \<Rightarrow> cmlp" where
+"AlphaExtSetD = undefined"
+
+definition AlphaParSetD ::
+  "'a fset cmle \<Rightarrow> ('a option \<Rightarrow> cmlp) \<Rightarrow> cmlp" where
+"AlphaParSetD = undefined"
+
+definition AlphaInlvSetD ::
+  "'a fset cmle \<Rightarrow> ('a option \<Rightarrow> cmlp) \<Rightarrow> cmlp" where
+"AlphaInlvSetD = undefined"
+
+definition HideD ::
+  "cmlp \<Rightarrow> cmlev set \<Rightarrow> cmlp" where
+"HideD p cs = undefined"
+
+definition InterruptD :: "cmlp \<Rightarrow> cmlp \<Rightarrow> cmlp" where
+"InterruptD p q = undefined"
+
+definition TimeoutD :: "cmlp \<Rightarrow> real cmle \<Rightarrow> cmlp \<Rightarrow> cmlp" where
+"TimeoutD p n q = undefined"
+
+definition WaitD :: "real cmle \<Rightarrow> cmlp" where
+"WaitD n = undefined"
 
 abbreviation MkChanD :: "string \<Rightarrow> 'a set \<Rightarrow> ('a option) CHAN" where
 "MkChanD n xs \<equiv> MkCHAN (bName n, TYPE('a option))"
@@ -41,6 +79,9 @@ abbreviation CommD :: "unit option CHAN \<Rightarrow> cmlp \<Rightarrow> cmlp" w
 (* FIXME: Execution of CML operations needs to take care of undefinedness *)
 
 (* FIXME: Surely these can all be unified into a single thing ... *)
+
+definition AssignC :: "'a cmlvar \<Rightarrow> 'a cmle \<Rightarrow> cmlp" where
+"AssignC x v = `\<lparr> defn(@v) \<rparr> \<turnstile> x := @v`"
 
 definition Exec0D :: "cmlp \<Rightarrow> cmlp" where
 "Exec0D p = p"
@@ -73,27 +114,75 @@ lift_definition Exec6D ::
    \<Rightarrow> 'a cmle \<Rightarrow> 'b cmle \<Rightarrow> 'c cmle \<Rightarrow> 'd cmle \<Rightarrow> 'e cmle \<Rightarrow> 'f cmle \<Rightarrow> cmlp" 
   is "\<lambda> P e f g h i j. {b :: cmlv binding. b \<in> P (e b) (f b) (g b) (h b) (i b) (j b)}" .
 
+definition IndexD :: "('a \<Rightarrow> cmlp) \<Rightarrow> 'a cmle \<Rightarrow> cmlp"
+where "IndexD F v = mkPRED {b. \<lbrakk>F(the(\<lbrakk>v\<rbrakk>\<^sub>*b))\<rbrakk>b}"
+
 (* We remove the standard definition of prefix and add one specific for CML *)
 
 no_syntax
   "_n_upred_prefixed"  :: "n_pexpr \<Rightarrow> n_upred \<Rightarrow> n_upred" ("_ -> _")
+  "_n_upred_index"         :: "('b \<Rightarrow> 'a upred) \<Rightarrow> 'b \<Rightarrow> n_upred" ("_<_>" 50)
 
 no_syntax (xsymbols)
   "_n_upred_prefixed"  :: "n_pexpr \<Rightarrow> n_upred \<Rightarrow> n_upred" ("_ \<rightarrow> _")
 
+nonterminal n_chanset and n_chan and n_chans
+
+syntax
+  "_n_chan_ev"       :: "idt => idt => n_chan"  ("_@_")
+  "_n_chan_ch"       :: "idt => n_chan" ("_")
+  "_n_chan"          :: "n_chan => n_chans" ("_")
+  "_n_chans"         :: "[n_chan, n_chans] => n_chans" ("_,/ _")
+  "_n_chanset_id"    :: "idt \<Rightarrow> n_chanset" ("_")
+  "_n_chanset_enum"  :: "n_chans => n_chanset" ("{|(_)|}")
+  "_n_chanset_union" :: "n_chanset \<Rightarrow> n_chanset \<Rightarrow> n_chanset" (infixl "union" 65)
+  "_n_chanset_inter" :: "n_chanset \<Rightarrow> n_chanset \<Rightarrow> n_chanset" (infixl "inter" 70)
+  "_n_chanset_diff"  :: "n_chanset \<Rightarrow> n_chanset \<Rightarrow> n_chanset" (infixl "\\" 70)
+
+translations
+  "_n_chan_ev c v"   => "CONST insert (CONST PEV c v) {}"
+  "_n_chan_ch c"     => "CONST MkEvents {c\<down>}"
+  "_n_chan cs"       => "cs"
+  "_n_chans cs1 cs2" => "cs1 \<union> cs2"
+  "_n_chanset_id x"    => "x"
+  "_n_chanset_enum cs" => "cs"
+  "_n_chanset_union cs1 cs2" => "cs1 \<union> cs2"
+  "_n_chanset_inter cs1 cs2" => "cs1 \<inter> cs2"
+  "_n_chanset_diff  cs1 cs2" => "cs1 - cs2"
+
 syntax
   "_n_upred_cml_prefix" :: "unit option CHAN \<Rightarrow> n_upred \<Rightarrow> n_upred" ("_ -> _")
-  "_n_upred_parcml"    :: "n_upred \<Rightarrow> cmlv UCHAN set \<Rightarrow> n_upred \<Rightarrow> n_upred" (infixl "[|_|]" 50)
-  "_n_upred_cml_exec0" :: "idt \<Rightarrow> n_upred" ("_'(')")
-  "_n_upred_cml_exec1" :: "idt \<Rightarrow> n_pexpr \<Rightarrow> n_upred" ("_'(_')")
-  "_n_upred_cml_exec2" :: "idt \<Rightarrow> n_pexpr \<Rightarrow> n_pexpr \<Rightarrow> n_upred" ("_'(_, _')")
-  "_n_upred_cml_exec3" :: "idt \<Rightarrow> n_pexpr \<Rightarrow> n_pexpr \<Rightarrow> n_pexpr \<Rightarrow> n_upred" ("_'(_, _, _')")
-  "_n_upred_cml_exec4" :: "idt \<Rightarrow> n_pexpr \<Rightarrow> n_pexpr \<Rightarrow> n_pexpr \<Rightarrow> n_pexpr \<Rightarrow> n_upred" ("_'(_, _, _, _')")
-  "_n_upred_cml_exec5" :: "idt \<Rightarrow> n_pexpr \<Rightarrow> n_pexpr \<Rightarrow> n_pexpr \<Rightarrow> n_pexpr \<Rightarrow> n_pexpr \<Rightarrow> n_upred" ("_'(_, _, _, _, _')")
-  "_n_upred_cml_exec6" :: "idt \<Rightarrow> n_pexpr \<Rightarrow> n_pexpr \<Rightarrow> n_pexpr \<Rightarrow> n_pexpr \<Rightarrow> n_pexpr \<Rightarrow> n_pexpr \<Rightarrow> n_upred" ("_'(_, _, _, _, _, _')")
+  "_n_upred_parcml"     :: "n_upred \<Rightarrow> n_chanset \<Rightarrow> n_upred \<Rightarrow> n_upred" (infixl "[|_|]" 50)
+  "_n_upred_aseqsetcml" :: "idt \<Rightarrow> n_pexpr \<Rightarrow> n_upred \<Rightarrow> n_upred" ("; _ in @set _ @ _")
+  "_n_upred_aextsetcml" :: "idt \<Rightarrow> n_pexpr \<Rightarrow> n_upred \<Rightarrow> n_upred" ("[] _ in @set _ @ _")
+  "_n_upred_aintsetcml" :: "idt \<Rightarrow> n_pexpr \<Rightarrow> n_upred \<Rightarrow> n_upred" ("|~| _ in @set _ @ _")
+  "_n_upred_aparsetcml" :: "idt \<Rightarrow> n_pexpr \<Rightarrow> n_upred \<Rightarrow> n_upred" ("|| _ in @set _ @ _")
+  "_n_upred_ainlvsetcml" :: "idt \<Rightarrow> n_pexpr \<Rightarrow> n_upred \<Rightarrow> n_upred" ("||| _ in @set _ @ _")
+  "_n_upred_hidecml"    :: "n_upred \<Rightarrow> n_chanset \<Rightarrow> n_upred" (infixl "\\" 60)
+  "_n_upred_intrptcml"  :: "n_upred \<Rightarrow> n_upred \<Rightarrow> n_upred" (infixl "'/-\\" 50)
+  "_n_upred_timeoutcml" :: "n_upred \<Rightarrow> n_pexpr \<Rightarrow> n_upred \<Rightarrow> n_upred" (infixl "['(_')>" 50)
+  "_n_upred_waitcml"    :: "n_pexpr \<Rightarrow> n_upred" ("WAIT _")
+  "_n_upred_cml_exec0"  :: "idt \<Rightarrow> n_upred" ("_'(')")
+  "_n_upred_cml_exec1"  :: "idt \<Rightarrow> n_pexpr \<Rightarrow> n_upred" ("_'(_')")
+  "_n_upred_cml_exec2"  :: "idt \<Rightarrow> n_pexpr \<Rightarrow> n_pexpr \<Rightarrow> n_upred" ("_'(_, _')")
+  "_n_upred_cml_exec3"  :: "idt \<Rightarrow> n_pexpr \<Rightarrow> n_pexpr \<Rightarrow> n_pexpr \<Rightarrow> n_upred" ("_'(_, _, _')")
+  "_n_upred_cml_exec4"  :: "idt \<Rightarrow> n_pexpr \<Rightarrow> n_pexpr \<Rightarrow> n_pexpr \<Rightarrow> n_pexpr \<Rightarrow> n_upred" ("_'(_, _, _, _')")
+  "_n_upred_cml_exec5"  :: "idt \<Rightarrow> n_pexpr \<Rightarrow> n_pexpr \<Rightarrow> n_pexpr \<Rightarrow> n_pexpr \<Rightarrow> n_pexpr \<Rightarrow> n_upred" ("_'(_, _, _, _, _')")
+  "_n_upred_cml_exec6"  :: "idt \<Rightarrow> n_pexpr \<Rightarrow> n_pexpr \<Rightarrow> n_pexpr \<Rightarrow> n_pexpr \<Rightarrow> n_pexpr \<Rightarrow> n_pexpr \<Rightarrow> n_upred" ("_'(_, _, _, _, _, _')")
+  "_n_upred_cindex"     :: "('b \<Rightarrow> 'a upred) \<Rightarrow> n_pexpr \<Rightarrow> n_upred" ("_<_>" 50)
+  
 
 translations
   "_n_upred_parcml p vs q"        == "CONST ParallelD p vs q"
+  "_n_upred_aseqsetcml x vs p"    == "CONST AlphaSeqSetD vs (\<lambda> x. p)"
+  "_n_upred_aintsetcml x vs p"    == "CONST AlphaIntSetD vs (\<lambda> x. p)"
+  "_n_upred_aextsetcml x vs p"    == "CONST AlphaExtSetD vs (\<lambda> x. p)"
+  "_n_upred_aparsetcml x vs p"    == "CONST AlphaParSetD vs (\<lambda> x. p)" 
+  "_n_upred_ainlvsetcml x vs p"   == "CONST AlphaInlvSetD vs (\<lambda> x. p)"
+  "_n_upred_hidecml p cs"         == "CONST HideD p cs"
+  "_n_upred_intrptcml p q"        == "CONST InterruptD p q"
+  "_n_upred_timeoutcml p n q"     == "CONST TimeoutD p n q"
+  "_n_upred_waitcml n"            == "CONST WaitD n"
   "_n_upred_cml_prefix n p"       == "CONST CommD n p"
   "_n_upred_cml_exec0 s"          == "CONST RH (CONST Exec0D s)"
   "_n_upred_cml_exec1 f s"        == "CONST RH (CONST Exec1D f s)"
@@ -102,10 +191,21 @@ translations
   "_n_upred_cml_exec3 v1 v2 v3 v4 s" == "CONST RH (CONST Exec3D v1 v2 v3 v4 s)"
   "_n_upred_cml_exec3 v1 v2 v3 v4 v5 s" == "CONST RH (CONST Exec3D v1 v2 v3 v4 v5 s)"
   "_n_upred_cml_exec3 v1 v2 v3 v4 v5 v6 s" == "CONST RH (CONST Exec3D v1 v2 v3 v4 v5 v6 s)"
+  "_n_upred_cindex F v"           == "CONST IndexD F v"
 
-term "`P [|{x,y,z}|] Q`"
+term "`|| i in @set {1,2,3} @ (P [(&i)> Q)`"
+term "`||| i in @set {1,2,3} @ (P [(&i)> Q)`"
+term "`; i in @set {1,2,3} @ (P [(&i)> Q)`"
+term "`[] i in @set {1,2,3} @ (P [(&i)> Q)`"
+term "`P [|{|x,y,z|}|] Q`"
+term "`P \\ {|x,y,z|}`"
+term "`P \\ {|x,y|} union {|z|}`"
+term "`P \\ xs`"
+term "`P /-\\ Q`"
+term "`P [(5)> Q`"
+term "`WAIT $x ; WAIT $y`"
 term "`f()`"
+term "`P<1>`"
 
-term "MkChanD"
 
 end
